2.  ùõçX = 3, ùõçY = 6
    $$
    C=
    \frac{1}{4}(
    \left[
    \begin{array}{}
    4 & 8 \\
    8 & 16
    \end{array}
    \right]+
    \left[
    \begin{array}{}
    1 & 2 \\
    2 & 4
    \end{array}
    \right]+
    \left[
    \begin{array}{}
    0 & 0 \\
    0 & 0
    \end{array}
    \right]+
    \left[
    \begin{array}{}
    1 & 2 \\
    2 & 4
    \end{array}
    \right]+\left[
    \begin{array}{}
    4 & 8 \\
    8 & 16
    \end{array}
    \right])
    $$
    $$
    C=\left[
    \begin{array}{}
    2.5 & 5 \\
    5 & 10
    \end{array}
    \right]
    $$

<br>

3.  
    $$
    \lvert A-
    \lambda I
    \rvert =0
    $$
    $$
    \begin{vmatrix}{}
    1-\lambda & 6 \\
    5 & 2-\lambda
    \end{vmatrix} = 0
    $$
    $$
    \lambda ^ 2 - 3 \lambda -28=0
    $$
    $$
    \lambda _1 = -4, \lambda _2 =7
    $$
    $$
    v_1 =
    \left[
    \begin{array}{}
    6a \\ -5a
    \end{array}
    \right],
    v_2 =
    \left[
    \begin{array}{}
    a \\ a
    \end{array}
    \right]
    $$

<br>

4.  (a) 
        $$
        V_N = (
        \frac{\sqrt{30}}{15},
        \frac{\sqrt{30}}{30},
        \frac{\sqrt{30}}{6}
        )
        $$
    (b)
        $$
        W_N = (
        \frac{5\sqrt{102}}{102},
        \frac{-\sqrt{102}}{34},
        \frac{4\sqrt{102}}{51},
        \frac{\sqrt{102}}{51}
        )
        $$
    (c)
        $$
        W_N = (
        \frac{1}{2},
        \frac{1}{2},
        \frac{1}{2},
        \frac{1}{2}
        )
        $$
    
<br>

5.  
    $$
    Z_{Jack}=
    \frac{48-60}{10}=-1.2
    $$
    $$
    Z_{Jill}=
    \frac{75-60}{10}=1.5
    $$

<br>

6.  
    (a) 
        $$
        \frac{189-155}{197-155}=
        \frac{17}{21}
        $$
    (b)
        $$
        \frac{169-155}{197-155}=
        \frac{1}{3}
        $$
    (c)
        $$
        \frac{1}{3}*(10-1)=3
        $$

<br>

7.  
    $$
    \lvert C-
    \lambda I
    \rvert =0
    $$
    $$
    \begin{vmatrix}{}
    {-2-\lambda} & -4 & 2 \\
    -2 & 1-\lambda & 2 \\
    4 & 2 & 5-\lambda
    \end{vmatrix} = 0
    $$
    $$
    (-2-\lambda)
    \begin{vmatrix}{}
    1-\lambda & 2 \\
    2 & 5-\lambda
    \end{vmatrix} - (-4)
    \begin{vmatrix}{}
    -2 & 2 \\
    4 & 5-\lambda
    \end{vmatrix} + 2
    \begin{vmatrix}{}
    -2 & 1-\lambda \\
    4 & 2
    \end{vmatrix}=0
    $$
    $$
    (-2-\lambda)
    (\lambda ^2-6\lambda+1) +4(2\lambda -18) + 2
    (4\lambda -8)=0
    $$
    $$
    (-\lambda ^3+4\lambda ^2+11\lambda -2)+
    16\lambda -88=0
    $$
    $$
    \lambda ^3-4\lambda ^2-27\lambda +90=0
    $$
    $$
    \lambda _1 = -5,
    \lambda _2 = 3,
    \lambda _3 = 6
    $$
    $$
    v_1 =
    \left[
    \begin{array}{}
    2a \\ a \\ -a
    \end{array}
    \right],
    v_2 =
    \left[
    \begin{array}{}
    2a \\ -a \\ -3a
    \end{array}
    \right]
    v_3 =
    \left[
    \begin{array}{}
    a \\ 2a \\ 8a
    \end{array}
    \right]
    $$
